PMapHelperLemmas.v
@@ -8,6 +8,7 @@ Require Import Coq.Lists.List.
 Require Import ZArith.
 
 Transparent lookup_ctrl.
+Transparent lookup_varlike_map.
 Lemma commute_lookup_eval_ctrl:
   forall c f s,
   lookup_ctrl (eval_sym_state s f) c =
@@ -19,7 +20,6 @@ Qed.
 
 (* Same as the above lemma for hdr and state *)
 Transparent lookup_hdr.
-Transparent lookup_hdr_map.
 Lemma commute_lookup_eval_hdr:
   forall h f s,
   lookup_hdr (eval_sym_state s f) h =
@@ -30,7 +30,6 @@ Proof.
 Qed.
 
 Transparent lookup_state.
-Transparent lookup_state_map.
 Lemma commute_lookup_eval_state:
   forall sv f s,
   lookup_state (eval_sym_state s f) sv =
@@ -86,6 +85,5 @@ Qed.
 
 Global Opaque lookup_hdr.
 Global Opaque lookup_state.
-Global Opaque lookup_hdr_map.
-Global Opaque lookup_state_map.
+Global Opaque lookup_varlike_map.
 Global Opaque lookup_ctrl.
